src/temporal_logic/refinement/one_to_one.lean
@@ -6,6 +6,7 @@ import ..spec
 universe variables u u₀ u₁ u₂
 open predicate nat
 local infix ` ≃ `:75 := v_eq
+local prefix `♯ `:0 := cast (by simp)
 
 namespace temporal
 
@@ -18,6 +19,7 @@ parameters {p : pred' (γ×α)} {q : pred' (γ×β)}
 parameters (A : evt → act (γ×α)) (C : evt → act (γ×β))
 parameters {cs₀ fs₀ : evt → pred' (γ×α)} {cs₁ fs₁ : evt → pred' (γ×β)}
 parameters (J : pred' (γ×α×β))
+parameters (Jₐ : pred' (γ×α))
 
 def C' (e : evt) : act (evt×γ×β) :=
 λ ⟨sch,s⟩ ⟨_,s'⟩, sch = e ∧ C e s s'
@@ -31,8 +33,7 @@ parameters p q cs₀ fs₀ cs₁ fs₁
 
 
 def SPEC₀.saf' (v : tvar α) (o : tvar γ) (sch : tvar evt) : cpred :=
-p ! ⦃ o,v ⦄ ⋀
-◻(∃∃ i, sch ≃ ↑i ⋀ ⟦ o,v | A i ⟧)
+spec_saf_spec p cs₀ fs₀ A ⦃o,v⦄ sch
 
 def SPEC₀ (v : tvar α) (o : tvar γ) : cpred :=
 spec p cs₀ fs₀ A ⦃o,v⦄
@@ -50,8 +51,13 @@ parameter SIM₀ : ∀ v o, (o,v) ⊨ q → ∃ w, (o,w) ⊨ p ∧ (o,w,v) ⊨ J
 parameter SIM
 : ∀ w v o v' o' e,
   (o,w,v) ⊨ J →
+  (o,w) ⊨ Jₐ →
+  (o,v) ⊨ cs₁ e →
+  (o,v) ⊨ fs₁ e →
   C e (o,v) (o',v') →
-  ∃ w', A e (o,w) (o',w') ∧
+  ∃ w', (o,w) ⊨ cs₀ e ∧
+        (o,w) ⊨ fs₀ e ∧
+        A e (o,w) (o',w') ∧
         (o',w',v') ⊨ J
 
 parameters (v : tvar β) (o : tvar γ) (sch : tvar evt)
@@ -59,6 +65,8 @@ parameters (v : tvar β) (o : tvar γ) (sch : tvar evt)
 variable (Γ : cpred)
 
 parameters β γ
+
+variable HJₐ : Γ ⊢ ∀∀ w, SPEC₀ w o ⟶ ◻(Jₐ ! ⦃o,w⦄)
 
 variable Hpo : ∀ w e sch,
   one_to_one_po' (SPEC₁ v o ⋀ SPEC₀.saf' w o sch ⋀ ◻(J ! ⦃o,w,v⦄))
@@ -73,15 +81,24 @@ open prod temporal.prod
 
 def Next_a : act $ (γ × evt) × α :=
 λ σ σ',
-∃ e, σ.1.2 = e ∧ (A e on map_left fst) σ σ'
+∃ e, σ.1.2 = e ∧
+     map_left fst σ ⊨ cs₀ e ∧
+     map_left fst σ ⊨ fs₀ e ∧
+     (A e on map_left fst) σ σ'
 
 def Next_c : act $ (γ × evt) × β :=
 λ σ σ',
-∃ e, σ.1.2 = e ∧ (C e on map_left fst) σ σ'
+∃ e, σ.1.2 = e ∧
+     map_left fst σ ⊨ cs₁ e ∧
+     map_left fst σ ⊨ fs₁ e ∧
+     (C e on map_left fst) σ σ'
 
 section J
 def J' : pred' ((γ × evt) × α × β) :=
 J ! ⟨ prod.map_left fst ⟩
+
+def JJₐ : pred' ((γ × evt) × α) :=
+Jₐ ! ⟨ prod.map_left fst ⟩
 
 def p' : pred' ((γ × evt) × α) :=
 p ! ⟨ prod.map_left fst ⟩
@@ -99,13 +116,13 @@ variable valid_witness
 : Γ ⊢ Wtn w
 
 lemma abstract_sch (e : evt)
-: Γ ⊢ sch ≃ e ⋀ ⟦ o,w | A e ⟧ ≡ sch ≃ e ⋀ ⟦ ⦃o,sch⦄,w | Next_a ⟧ :=
+: Γ ⊢ sch ≃ e ⋀ cs₀ e ! ⦃o,w⦄ ⋀ fs₀ e ! ⦃o,w⦄ ⋀ ⟦ o,w | A e ⟧ ≡
+      sch ≃ e ⋀ ⟦ ⦃o,sch⦄,w | Next_a ⟧ :=
 begin
   lifted_pred,
   split ; intro h ; split
-  ; cases h with h₀ h₁ ; try { assumption },
-  { simp [Next_a,on_fun,h₀], auto, },
-  { simp [Next_a,on_fun,h₀] at h₁, auto }
+  ; casesm* _ ∧ _ ; try { assumption }
+  ; simp [Next_a,on_fun] at * ; cc,
 end
 
 section Simulation_POs
@@ -126,16 +143,20 @@ omit SIM₀
 include SIM
 lemma SIM' (w : α) (v : β) (o : γ × evt) (v' : β) (o' : γ × evt)
   (h₀ : (o, w, v) ⊨ J')
-  (h₁ : Next_c (o, v) (o', v'))
+  (h₃ : (o, w) ⊨ JJₐ)
+  (h₄ : Next_c (o, v) (o', v'))
 : (∃ w', Next_a (o,w) (o',w') ∧ (o', w', v') ⊨ J') :=
 begin
   simp [J',map] at h₀,
-  simp [Next_c,on_fun] at h₁,
-  specialize SIM w v o.1 v' o'.1 o.2 h₀ h₁,
+  simp [Next_c,on_fun] at h₄,
+  casesm* _ ∧ _,
+  simp [JJₐ] at h₃,
+  specialize SIM w v o.1 v' o'.1 o.2 h₀ _ _ _ _
+  ; try { assumption },
   cases SIM with w' SIM,
   existsi [w'],
   simp [Next_a, J',on_fun,map,h₀],
-  exact SIM,
+  tauto,
 end
 
 include H
@@ -146,12 +167,11 @@ begin [temporal]
   simp [SPEC₂,simulation.SPEC₁,q'] at H ⊢,
   split, tauto,
   casesm* _ ⋀ _,
-  persistent,
   select h : ◻p_exists _,
-  henceforth at h ⊢,
+  henceforth! at h ⊢,
   cases h with e h,
   explicit' [Next_c,sched]
-  { cc }
+  { casesm* _ ∧ _, subst e, tauto, }
 end
 
 include SIM₀ SIM
@@ -160,12 +180,21 @@ lemma witness_imp_SPEC₀_saf
 : Γ ⊢ SPEC₀.saf' w o sch :=
 begin [temporal]
   have hJ := J_inv_in_w p' q'
-                        temporal.one_to_one.Next_a temporal.one_to_one.Next_c
+                        temporal.one_to_one.Next_a
+                        temporal.one_to_one.Next_c
                         temporal.one_to_one.J'
+                        temporal.one_to_one.JJₐ
                         temporal.one_to_one.SIM₀'
                         temporal.one_to_one.SIM'
                         v ⦃o,sch⦄ Γ
                         (temporal.one_to_one.H' _ H) _ h,
+  have hJ' := abs_J_inv_in_w p' q'--
+                        temporal.one_to_one.Next_a
+                        temporal.one_to_one.J'
+                        temporal.one_to_one.JJₐ
+                        temporal.one_to_one.SIM₀'
+                        v ⦃o,sch⦄ Γ
+                        _ h ,
   simp [SPEC₀.saf',SPEC₂,Wtn,simulation.Wtn] at h ⊢ H,
   casesm* _ ⋀ _,
   split,
@@ -181,18 +210,15 @@ begin [temporal]
   { clear SIM₀,
     select h : ◻(_ ≃ _),
     select h' : ◻(p_exists _),
-    persistent,
-    henceforth at h h' ⊢ hJ,
-    explicit
-    { existsi σ ⊨ sch,
-      simp at ⊢ h,
-      repeat
-      { unfold_coes at h <|>
-        simp [Wf,Wf_f,J',map] at h hJ },
-      simp at h h',
-      simp [Next_a,on_fun,map_right] at h,
-      rw [h], clear h,
-      apply_epsilon_spec, } },
+    henceforth! at h h' ⊢ hJ hJ',
+    explicit' [Wf,Wf_f,J',JJₐ]
+    { simp [Next_a,on_fun] at h h',
+      casesm* [_ ∧ _,Exists _],
+      subst w', subst h'_w,
+      apply_epsilon_spec,
+      have : (∃ (w' : α), (o, w) ⊨ cs₀ sch ∧
+      (o, w) ⊨ fs₀ sch ∧ A sch (o, w) (o', w') ∧ (o', w', v') ⊨ J), auto,
+      cases this, tauto, } },
 end
 
 omit H
@@ -204,8 +230,8 @@ lemma SPEC₂_imp_SPEC₁
 begin [temporal]
   simp only [SPEC₁,SPEC₂,temporal.one_to_one.SPEC₁,temporal.one_to_one.SPEC₂],
   monotonicity, apply ctx_p_and_p_imp_p_and',
-  { monotonicity, simp, intros x h₀ h₁,
-    existsi x, exact h₁ },
+  { monotonicity, simp, intros x h₀ h₁ _ _,
+    existsi x, tauto, },
   { intros h i h₀ h₁,
     replace h := h _ h₀ h₁,
     revert h, monotonicity, simp, }
@@ -213,7 +239,7 @@ end
 
 lemma H_C_imp_A (e : evt)
 : SPEC₂ v o sch ⋀ Wtn w ⋀ ◻(J ! ⦃o,w,v⦄) ⟹
-  ◻(sch ≃ ↑e ⋀ ⟦ o,v | C e ⟧ ⟶ ⟦ o,w | A e ⟧) :=
+  ◻(cs₁ e ! ⦃o,v⦄ ⋀ fs₁ e ! ⦃o,v⦄ ⋀ sch ≃ ↑e ⋀ ⟦ o,v | C e ⟧ ⟶ cs₀ e ! ⦃o,w⦄ ⋀ fs₀ e ! ⦃o,w⦄ ⋀ ⟦ o,w | A e ⟧) :=
 begin [temporal]
   intro H',
   have H : temporal.one_to_one.SPEC₁ v o ⋀
@@ -227,19 +253,19 @@ begin [temporal]
   let J' := temporal.one_to_one.J',
   have SIM₀' := temporal.one_to_one.SIM₀', clear SIM₀,
   have SIM' := temporal.one_to_one.SIM',  clear SIM,
-  have := C_imp_A_in_w p' _ (Next_a A) (Next_c C) J' SIM₀' SIM' v ⦃o,sch⦄ Γ _ w _,
-  { persistent, henceforth at this ⊢,
-    simp, intros h₀ h₁, clear_except this h₀ h₁,
-    suffices : sch ≃ ↑e ⋀ ⟦ o,w | A e ⟧, apply this.right,
+  have := C_imp_A_in_w p' _ (Next_a A) (Next_c C) J' _ SIM₀' SIM' v ⦃o,sch⦄ Γ _ w _,
+  { henceforth! at this ⊢,
+    simp, intros h₀ h₁ h₂ h₃, clear_except this h₀ h₁ h₂ h₃,
+    suffices : sch ≃ ↑e ⋀ cs₀ e ! ⦃o,w⦄ ⋀ fs₀ e ! ⦃o,w⦄ ⋀ ⟦ o,w | A e ⟧, admit,
     rw abstract_sch, split, assumption,
     apply this _,
     simp [Next_c],
     suffices : ⟦ ⦃o,sch⦄,v | λ (σ σ' : (γ × evt) × β), (σ.fst).snd = e ∧ (C e on map_left fst) σ σ' ⟧,
-    { revert this, action { simp, intro, subst e, simp, },  },
+    { explicit' { cc, }, },
     rw [← action_and_action,← init_eq_action,action_on'], split,
     explicit
     { simp at ⊢ h₀, assumption },
-    simp [h₁], },
+    simp [h₃], },
   clear_except H',
   simp [simulation.SPEC₁,SPEC₂,temporal.one_to_one.SPEC₂] at H' ⊢,
   cases_matching* _ ⋀ _, split,
@@ -248,8 +274,8 @@ begin [temporal]
     henceforth at H' ⊢, cases H' with i H',
     simp [Next_c],
     suffices : ⟦ ⦃o,sch⦄,v | λ (σ σ' : (γ × evt) × β), (σ.fst).snd = i ∧ (C i on map_left fst) σ σ' ⟧,
-    { revert this, action { simp, intro, subst i, simp } },
-    rw [← action_and_action], },
+    { explicit' { cases this, subst i, tauto, } },
+    explicit' { cc }, },
   { cases_matching* _ ⋀ _, assumption, },
 end
 
@@ -278,8 +304,14 @@ begin
     simp at *,
     transitivity,
     { apply this },
-    { assumption } },
-  apply temporal.one_to_one.H_C_imp_A Hpo w e,
+    { assumption }, },
+  begin [temporal]
+    intros Hs,
+    have H_imp := temporal.one_to_one.H_C_imp_A Hpo w e _ Hs,
+    henceforth! at ⊢ H_imp,
+    simp at H_imp ⊢,
+    exact H_imp,
+  end
 end
 
 end Simulation_POs
@@ -289,13 +321,14 @@ include H SIM₀ SIM Hpo
 lemma sched_ref (i : evt) (w : tvar α)
  (Hw : Γ ⊢ Wtn w)
  (h : Γ ⊢ sched (cs₁ i ! ⦃o,v⦄) (fs₁ i ! ⦃o,v⦄) (sch ≃ ↑i ⋀ ⟦ o,v | C i ⟧))
-: Γ ⊢ sched (cs₀ i ! ⦃o,w⦄) (fs₀ i ! ⦃o,w⦄) ⟦ o,w | A i ⟧ :=
+: Γ ⊢ sched (cs₀ i ! ⦃o,w⦄) (fs₀ i ! ⦃o,w⦄)
+            ⟦ o,w | A i ⟧ :=
 begin [temporal]
   have H' := one_to_one.H' C v o sch _ H,
   have hJ : ◻(J' J ! ⦃⦃o,sch⦄,w,v⦄),
   { replace SIM₀ := SIM₀' _ SIM₀,
-    replace SIM := SIM' A C J SIM,
-    apply simulation.J_inv_in_w p' q' (Next_a A) _ (J' J) SIM₀ SIM _ ⦃o,sch⦄ _ H' w Hw },
+    replace SIM := SIM' A C J _ SIM,
+    apply simulation.J_inv_in_w p' q' (Next_a A) _ (J' J) _ SIM₀ SIM _ ⦃o,sch⦄ _ H' w Hw, },
   simp [J'] at hJ,
   have Hpo' := temporal.one_to_one.Hpo' Hpo w i,
   apply replacement Hpo' Γ _,
@@ -312,34 +345,33 @@ begin [temporal]
   apply ctx_p_and_p_imp_p_and' _ _,
   apply ctx_p_and_p_imp_p_and' _ _,
   { clear_except SIM₀ Hw H,
-    replace SIM₀ := SIM₀' _ SIM₀,
-    have := init_in_w p' q' (Next_a A) (J' J) SIM₀ v ⦃o,sch⦄ Γ,
+    replace SIM₀ := temporal.one_to_one.SIM₀',
+    have := init_in_w p' q' (Next_a A) (J' J) SIM₀ v ⦃o,sch⦄ Γ _ Hw,
     intro Hq,
-    replace this := this _ Hw _, simp [p'] at this,
-    apply this,
-    simp [q',proj_assoc], apply Hq, },
+    simp [p',q'] at this,
+    auto, },
   { clear_except SIM SIM₀ Hw H,
     have H' := H' C v o sch _ H,
     replace SIM₀ := SIM₀' _ SIM₀,
-    replace SIM := SIM' A C J SIM,
+    replace SIM := SIM' A C J _ SIM,
     have := temporal.simulation.C_imp_A_in_w p' q'
-      (Next_a A) (Next_c C) (J' J) SIM₀ SIM v ⦃o,sch⦄ _ H' w Hw,
+      (Next_a A) (Next_c C) (J' J) _ SIM₀ SIM v ⦃o,sch⦄ _ H' w Hw,
     { monotonicity!,
       simp [exists_action],
-      intros e h₀ h₁, replace this := this _,
-      { revert this,
-        explicit { simp [Next_a,on_fun], intros h, exact ⟨_,h⟩ }, },
+      intros e h₀ h₁ h₂ h₃, replace this := this _,
+      explicit' [Next_a]
+      { intros, casesm* _ ∧ _,
+        constructor_matching* [Exists _,_ ∧ _] ; auto, },
       simp [Next_c],
-      suffices : ⟦ ⦃o,sch⦄,v | λ (σ σ' : (γ × evt) × β), ((λ s s', s = e) on (prod.snd ∘ prod.fst)) σ σ' ∧ (C e on map_left prod.fst) σ σ' ⟧,
-      revert this, action
-      { simp [function.on_fun],
-        intros, subst e, assumption, },
-      rw ← action_and_action, simp,
-      rw [action_on,action_on,coe_over_comp,proj_assoc,← init_eq_action,coe_eq],
-      simp, split ; assumption } },
+      suffices : ⟦ ⦃o,sch⦄,v | λ (σ σ' : (γ × evt) × β), map_left prod.fst σ ⊨ fs₁ e ∧ ((λ s s', s = e) on (prod.snd ∘ prod.fst)) σ σ' ∧ (C e on map_left prod.fst) σ σ' ⟧,
+      explicit'
+      { intros, subst e, tauto, },
+      henceforth at this,
+      explicit' [Next_c]
+      { tauto } } },
   { intros h i,
     replace h := h i,
-    apply temporal.one_to_one.sched_ref ; auto },
+    apply temporal.one_to_one.sched_ref; auto },
 end
 end SPEC₂
 
@@ -351,7 +383,7 @@ lemma refinement_SPEC₂
 : Γ ⊢ (∃∃ sch, SPEC₂ v o sch) ⟶ (∃∃ a, SPEC₀ a o) :=
 begin [temporal]
   simp, intros sch Hc,
-  apply one_to_one A C J SIM₀ SIM _ _ _ _ _  Hc,
+  apply one_to_one A C J Jₐ SIM₀ SIM _ _ _ _ _  Hc,
   apply Hpo,
 end
 end refinement_SPEC₂
@@ -374,7 +406,7 @@ begin [temporal]
     apply refinement_SPEC₁, },
   { simp, intros c sch Hspec,
     specialize h c, simp [one_to_one_po'] at h,
-    apply refinement_SPEC₂ A C cs₀ fs₀ cs₁ fs₁ J SIM₀ SIM c o _ _ _,
+    apply refinement_SPEC₂ A C cs₀ fs₀ cs₁ fs₁ J Jₐ SIM₀ SIM c o _ _ _,
     simp [one_to_one_po'],
     exact h,
     existsi sch, assumption },
