src/temporal_logic/spec.lean
@@ -13,15 +13,20 @@ variables (cs fs : evt → pred' α)
 variables (A : evt → act α)
 
 @[simp]
+def spec_saf_spec (v : tvar α) (sch : tvar evt) : cpred :=
+p ! v ⋀
+◻(∃∃ e, sch ≃ ↑e ⋀ cs e ! v ⋀ fs e ! v ⋀ ⟦ v | A e ⟧)
+
+@[simp]
 def spec (v : tvar α) : cpred :=
 p ! v ⋀
-◻(∃∃ e, ⟦ v | A e ⟧) ⋀
+◻(∃∃ e, cs e ! v ⋀ fs e ! v ⋀ ⟦ v | A e ⟧) ⋀
 ∀∀ e, sched (cs e ! v) (fs e ! v) ⟦ v | A e ⟧
 
 @[simp]
 def spec_sch (v : tvar α) (sch : tvar evt) : cpred :=
 p ! v ⋀
-◻(∃∃ e, sch ≃ ↑e ⋀ ⟦ v | A e ⟧) ⋀
+◻(∃∃ e, sch ≃ ↑e ⋀ cs e ! v ⋀ fs e ! v ⋀ ⟦ v | A e ⟧) ⋀
 ∀∀ e, sched (cs e ! v) (fs e ! v) (sch ≃ e ⋀ ⟦ v | A e ⟧)
 
 
